Otway-Rees: implemented serialization and parsing of encrypted message parts

otway-rees/OYRS.Messages.fst
@@ -4,12 +4,85 @@ module OYRS.Messages
 module LC = LabeledCryptoAPI
 
 
+let valid_encval i ev l =
+  match ev with
+  | EncMsg1 n_a c a b -> is_msg i n_a l /\ is_msg i c l
+  | EncMsg2 n_b c a b -> is_msg i n_b l /\ is_msg i c l
+  | EncMsg3_I n_a k_ab -> is_msg i n_a l /\ is_msg i k_ab l
+  | EncMsg3_R n_b k_ab -> is_msg i n_b l /\ is_msg i k_ab l
+
+let serialize_encval i ev l =
+  match ev with
+  | EncMsg1 n_a c a b ->
+    let tag = LC.string_to_bytes #oyrs_global_usage #i "ev1" in
+    let a_bytes = LC.string_to_bytes #oyrs_global_usage #i a in
+    let b_bytes = LC.string_to_bytes #oyrs_global_usage #i b in
+    LC.concat #oyrs_global_usage #i #l tag (LC.concat #oyrs_global_usage #i #l n_a (LC.concat #oyrs_global_usage #i #l c (LC.concat #oyrs_global_usage #i #l a_bytes b_bytes)))
+  | EncMsg2 n_b c a b ->
+    let tag = LC.string_to_bytes #oyrs_global_usage #i "ev2" in
+    let a_bytes = LC.string_to_bytes #oyrs_global_usage #i a in
+    let b_bytes = LC.string_to_bytes #oyrs_global_usage #i b in
+    LC.concat #oyrs_global_usage #i #l tag (LC.concat #oyrs_global_usage #i #l n_b (LC.concat #oyrs_global_usage #i #l c (LC.concat #oyrs_global_usage #i #l a_bytes b_bytes)))
+  | EncMsg3_I n_a k_ab ->
+    let tag = LC.string_to_bytes #oyrs_global_usage #i "ev3_i" in
+    LC.concat #oyrs_global_usage #i #l tag (LC.concat #oyrs_global_usage #i #l n_a k_ab)
+  | EncMsg3_R n_b k_ab ->
+    let tag = LC.string_to_bytes #oyrs_global_usage #i "ev3_r" in
+    LC.concat #oyrs_global_usage #i #l tag (LC.concat #oyrs_global_usage #i #l n_b k_ab)
+
+let parse_encval #i #l (sev:msg i l) =
+  LC.split #oyrs_global_usage #i #l sev `bind` (fun r1 ->
+  let (tag_bytes, rest) = r1 in
+  LC.bytes_to_string #oyrs_global_usage #i tag_bytes `bind` (fun tag ->
+  match tag with
+  | "ev1" -> (
+    LC.split #oyrs_global_usage #i #l rest `bind` (fun r2 ->
+    let (n_a, rest) = r2 in
+    LC.split #oyrs_global_usage #i #l rest `bind` (fun r3 ->
+    let (c, rest) = r3 in
+    LC.split #oyrs_global_usage #i #l rest `bind` (fun r4 ->
+    let (a_bytes, b_bytes) = r4 in
+    LC.bytes_to_string #oyrs_global_usage #i a_bytes `bind` (fun a ->
+    LC.bytes_to_string #oyrs_global_usage #i b_bytes `bind` (fun b ->
+    Success (EncMsg1 n_a c a b)
+    )))))
+  )
+  | "ev2" -> (
+    LC.split #oyrs_global_usage #i #l rest `bind` (fun r2 ->
+    let (n_b, rest) = r2 in
+    LC.split #oyrs_global_usage #i #l rest `bind` (fun r3 ->
+    let (c, rest) = r3 in
+    LC.split #oyrs_global_usage #i #l rest `bind` (fun r4 ->
+    let (a_bytes, b_bytes) = r4 in
+    LC.bytes_to_string #oyrs_global_usage #i a_bytes `bind` (fun a ->
+    LC.bytes_to_string #oyrs_global_usage #i b_bytes `bind` (fun b ->
+    Success (EncMsg2 n_b c a b)
+    )))))
+  )
+  | "ev3_i" -> (
+    LC.split #oyrs_global_usage #i #l rest `bind` (fun r2 ->
+    let (n_a, k_ab) = r2 in
+    Success (EncMsg3_I n_a k_ab)
+    )
+  )
+  | "ev3_r" -> (
+    LC.split #oyrs_global_usage #i #l rest `bind` (fun r2 ->
+    let (n_b, k_ab) = r2 in
+    Success (EncMsg3_R n_b k_ab)
+    )
+  )
+  | t -> Error ("invalid tag: " ^ t)
+  ))
+
+let parse_serialize_encval_lemma i ev l = ()
+
+
 let valid_message i m =
   match m with
-  | Msg1 c a b ev_a -> LC.is_msg oyrs_global_usage i c public
-  | Msg2 c a b ev_a ev_b -> LC.is_msg oyrs_global_usage i c public
-  | Msg3 c ev_a ev_b -> LC.is_msg oyrs_global_usage i c public
-  | Msg4 c ev_a -> LC.is_msg oyrs_global_usage i c public
+  | Msg1 c a b ev_a -> is_msg i c public
+  | Msg2 c a b ev_a ev_b -> is_msg i c public
+  | Msg3 c ev_a ev_b -> is_msg i c public
+  | Msg4 c ev_a -> is_msg i c public
 
 let serialize_msg i m =
   match m with
